src/impl/TLS13.Impl.Server.fsti
@@ -97,6 +97,29 @@ let next_local_action_sound
          CL.message_value =
            M.TlsHandshake (M.EncryptedExtensions { M.negotiated_alpn = None });
        })
+    | ST.LocalSendCertificateVerify ->
+     action.ST.next_local_payload == ST.LocalPayloadNone /\
+     st.CS.cs_model.CS.model_control ==
+       CS.ControlHandshaking CS.HsServerEncryptedFlightSent /\
+     st.CS.cs_model.CS.model_config.CS.config_role == CS.ServerEndpoint /\
+     st.CS.cs_model.CS.model_handshake.CS.hs_certificate <> None /\
+     st.CS.cs_model.CS.model_handshake.CS.hs_certificate_verify_verified /\
+     Some? st.CS.cs_model.CS.model_handshake.CS.hs_certificate_verify /\
+     Some?
+       st.CS.cs_model.CS.model_handshake.CS.hs_keys.CS.ks_server_handshake_traffic /\
+     U64.fits
+       (st.CS.cs_model.CS.model_record.CS.record_write.R.seq + 1) /\
+     (let cv = Some?.v
+        st.CS.cs_model.CS.model_handshake.CS.hs_certificate_verify in
+      B.length st.CS.cs_model.CS.model_handshake.CS.hs_transcript +
+        B.length (TLS13.Wire.Spec.serialize_certificate_verify_from_signature cv) <=
+          Bounds.max_transcript_len /\
+      CS.legal_event
+        st.CS.cs_model
+        (CS.ConnNetworkEvent {
+          CL.message_direction = CL.Sent;
+          CL.message_value = M.TlsHandshake (M.CertificateVerify cv);
+        }))
     | _ ->
      False
   else
